more loc_transform lemmas

CCsub_LocTransform.v
@@ -19,20 +19,19 @@ Proof with eauto.
   intros * EnvTyp WfCtx LocTrans.
   generalize dependent Γ.
   dependent induction LocTrans; intros; subst; simpl in *...
-  { inverts EnvTyp; simpl_env in WfCtx... }
-  inverts EnvTyp.
+  { inversion EnvTyp; subst; simpl_env in WfCtx... }
+  inversion EnvTyp; subst.
   eapply IHLocTrans...
   eapply wf_ctx_subst_cb...
 Qed.
 
 Lemma loc_transform_cse_ident : forall E C,
-  cse_fvars C = {}A ->
+  (forall x, x `notin`A cse_fvars C) ->
   loc_transform_cse E C C.
 Proof with eauto.
   intros * Fv.
   induction E...
   destruct a as [x l].
-  assert (x `notin` cse_fvars C) by (rewrite Fv; fsetdec).
   apply loc_transform_cse_multi with (E := E) (C := C)...
   simpl_env.
   rewrite <- subst_cse_fresh...
@@ -40,7 +39,7 @@ Qed.
 
 Lemma loc_transform_cse_result : forall C E,
   exists C2, loc_transform_cse E C C2.
-Proof with eauto*.
+Proof with eauto.
   intros.
   generalize dependent C.
   dependent induction E; intros...
@@ -53,7 +52,7 @@ Lemma loc_transform_cse_deterministic : forall E C1 C2 C3,
   loc_transform_cse E C1 C2 ->
   loc_transform_cse E C1 C3 ->
   C2 = C3.
-Proof with eauto*.
+Proof with eauto.
   intros * LocTrans1 LocTrans2.
   generalize dependent C3.
   dependent induction LocTrans1; intros; subst; simpl in *.
@@ -62,13 +61,12 @@ Proof with eauto*.
 Qed.
 
 Lemma loc_transform_ident : forall E T,
-  fv_ct T = {}A ->
+  (forall x, x `notin`A fv_ct T) ->
   loc_transform E T T.
 Proof with eauto.
   intros * Fv.
   induction E...
   destruct a as [x l].
-  assert (x `notin` fv_ct T) by (rewrite Fv; fsetdec).
   apply loc_transform_multi with (E := E) (T := T)...
   rewrite <- subst_ct_fresh...
 Qed.
@@ -77,7 +75,7 @@ Lemma loc_transform_deterministic : forall E T1 T2 T3,
   loc_transform E T1 T2 ->
   loc_transform E T1 T3 ->
   T2 = T3.
-Proof with eauto*.
+Proof with eauto.
   intros * LocTrans1 LocTrans2.
   generalize dependent T3.
   dependent induction LocTrans1; intros; subst; simpl in *.
@@ -86,7 +84,7 @@ Qed.
 
 Lemma loc_transform_result : forall T E,
   exists T2, loc_transform E T T2.
-Proof with eauto*.
+Proof with eauto.
   intros *.
   generalize dependent T.
   dependent induction E; intros; simpl in *.
@@ -111,13 +109,12 @@ Qed.
 Lemma subst_ct_invert_capt : forall T C R D x,
   subst_ct x D T = C # R ->
   exists C' R', T = C' # R' /\ C = subst_cse x D C' /\ R = subst_ct x D R'.
-Proof with eauto*.
+Proof with eauto.
   intros * Eq.
   generalize dependent C.
   generalize dependent R.
-  induction T; simpl in *; intros...
-  destruct v...
-  exists c, T; repeat split...
+  induction T; simpl in *; intros; try inversion Eq...
+  destruct v; inversion Eq.
 Qed.
 
 Lemma loc_transform_capt : forall E C R T,
@@ -133,7 +130,7 @@ Qed.
 Lemma loc_tranform_equiv : forall E C R C' R',
   loc_transform E (C # R) (C' # R') <->
   (loc_transform E R R' /\ loc_transform_cse E C C').
-Proof with eauto*.
+Proof with eauto.
   intros *.
   split; intros LocTrans.
   - dependent induction LocTrans; simpl in *...
@@ -155,7 +152,7 @@ Proof with eauto.
   intros * EnvTyp WfCse LocTrans.
   generalize dependent Γ.
   dependent induction LocTrans; simpl in *; eauto; intros Γ EnvTyp WfCse; subst.
-  - inverts EnvTyp...
+  - inversion EnvTyp; subst...
   - inversion EnvTyp; subst.
     eapply IHLocTrans; eauto.
     rewrite_env (nil ++ [(x, bind_typ (cse_loc l # R))] ++ Γ0) in WfCse.
@@ -165,67 +162,6 @@ Proof with eauto.
     apply H0...
 Qed.
 
-Lemma bind_typ_capt : forall x Γ S T,
-  wf_ctx Γ S ->
-  binds x (bind_typ T) Γ ->
-  exists C R,
-    T = C # R.
-Proof with eauto*.
-  intros * WfCtx Binds.
-  dependent induction WfCtx; intros; simpl in *.
-  - inversion Binds.
-  - simpl_env in Binds.
-    binds_cases Binds; subst; simpl in *.
-    destruct (IHWfCtx H2) as [C [R Eq]]; subst...
-  - simpl_env in Binds.
-    binds_cases Binds; subst; simpl in *.
-    destruct (IHWfCtx H1) as [C1 [R1 Eq]]; subst...
-    inverts H3...
-Qed.
-
-Lemma runtime_ctx_binds_loc : forall Γ E S x C R,
-  env_well_typed S E Γ ->
-  binds x (bind_typ (C # R)) Γ ->
-  exists l, binds x l E /\ C = cse_loc l.
-Proof with eauto*.
-  intros * EnvTyp Binds.
-  dependent induction EnvTyp; intros; simpl in *.
-  { inversion Binds. }
-  simpl_env in Binds.
-  binds_cases Binds; subst; simpl in *.
-  - destruct (IHEnvTyp H1) as [l0 [BindsL0 Eq]]; subst.
-    exists l0; split...
-    simpl_env.
-    eapply binds_tail...
-  - inverts H3.
-    exists l; split...
-    simpl_env.
-    eapply binds_head...
-Qed.
-
-Lemma wf_cse_empty_means_no_fvars : forall C S,
-  wf_cse nil S C ->
-  cse_fvars C = {}A.
-Proof with eauto.
-  intros * WfCse.
-  dependent induction WfCse; simpl in *; eauto.
-  - inversion H.
-  - rewrite IHWfCse1, IHWfCse2...
-    fsetdec...
-Qed.
-
-Lemma wf_typ_empty_means_no_fvars : forall T S,
-  wf_typ nil S T ->
-  fv_ct T = {}A.
-Proof with eauto.
-  intros * WfTyp.
-  enough (fv_ct T `subset` {}A) by fsetdec.
-  unfold AtomSet.F.Subset in *.
-  intros.
-  epose proof (wf_typ_notin_fv_ct a _ _ _ WfTyp)...
-  simpl in *.
-  assert (a `in` fv_ct T -> a `in` {}A) by fsetdec...
-Qed.
 
 Lemma loc_transform_cse_join : forall E C1 C2 C1' C2',
   loc_transform_cse E C1 C1' ->
@@ -241,26 +177,30 @@ Proof with eauto.
 Qed.
 
 Lemma loc_transform_cse_bound_fvar : forall E x l,
+  uniq E ->
   binds x l E ->
   loc_transform_cse E (cse_fvar x) (cse_loc l).
 Proof with eauto.
-  intros * Binds.
+  intros * Uniq Binds.
   induction E; simpl in *...
   { inversion Binds. }
   destruct a as [y l'].
   simpl_env in Binds.
-  binds_cases Binds; subst; simpl in *.
-  - assert (x <> y) by fsetdec.
-    constructor...
-    rewrite <- subst_cse_fresh...
+  analyze_binds Binds.
   - constructor...
     simpl...
-    destruct (x == x); try fsetdec...
+    destruct (y == y); try fsetdec...
     epose proof (loc_transform_cse_ident E (cse_loc l'))...
+  - inversion Uniq; subst.
+    constructor...
+    rewrite <- subst_cse_fresh...
+    simpl.
+    enough (y <> x) by fsetdec.
+    intro; subst...
 Qed.
 
 Lemma loc_transform_cse_unbound_fvar : forall E x,
-  x `notin` dom E ->
+  x `notin`A dom E ->
   loc_transform_cse E (cse_fvar x) (cse_fvar x).
 Proof with eauto.
   intros * NotIn.
@@ -277,8 +217,25 @@ Ltac loc_transform_cse_ident_eq H :=
       unshelve epose proof (loc_transform_cse_deterministic _ _ _ _ H (loc_transform_cse_ident E C _)); subst
   end.
 
-Lemma loc_transform_ctx_binds : forall E Δ Δ' x T U,
-  x `notin` dom E ->
+Ltac loc_transform_ident_eq H :=
+  match type of H with
+  | loc_transform ?E ?T ?T' =>
+      unshelve epose proof (loc_transform_deterministic _ _ _ _ H (loc_transform_ident E T _)); subst
+  end.
+
+Lemma loc_transform_unbound_var : forall E X,
+  X `notin`A dom E ->
+  loc_transform E X X.
+Proof with eauto.
+  intros * NotIn.
+  induction E; simpl in *...
+  destruct a as [y l].
+  assert (X <> y) by fsetdec.
+  constructor...
+Qed.
+
+Lemma loc_transform_ctx_binds_typ : forall E Δ Δ' x T U,
+  x `notin`A dom E ->
   loc_transform_ctx E Δ Δ' ->
   binds x (bind_typ T) Δ ->
   loc_transform E T U ->
@@ -287,9 +244,26 @@ Proof with eauto.
   intros * NotIn LocTrans Binds LocTransT.
   generalize dependent T.
   generalize dependent U.
-  dependent induction LocTrans; intros; subst; simpl in *; inverts LocTransT...
+  dependent induction LocTrans; intros; subst; simpl in *; inversion LocTransT; subst...
   destruct (x == x0); try fsetdec...
-  assert (x `notin` dom E) by fsetdec.
+  assert (x `notin`A dom E) by fsetdec.
+  eapply IHLocTrans; eauto.
+  replace (bind_typ (subst_ct x0 (cse_loc l) T)) with (subst_cb x0 (cse_loc l) (bind_typ T))...
+Qed.
+
+Lemma loc_transform_ctx_binds_sub : forall E Δ Δ' x T U,
+  x `notin`A dom E ->
+  loc_transform_ctx E Δ Δ' ->
+  binds x (bind_sub T) Δ ->
+  loc_transform E T U ->
+  binds x (bind_sub U) Δ'.
+Proof with eauto.
+  intros * NotIn LocTrans Binds LocTransT.
+  generalize dependent T.
+  generalize dependent U.
+  dependent induction LocTrans; intros; subst; simpl in *; inversion LocTransT; subst...
+  destruct (x == x0); try fsetdec...
+  assert (x `notin`A dom E) by fsetdec.
   eapply IHLocTrans; eauto.
   replace (bind_typ (subst_ct x0 (cse_loc l) T)) with (subst_cb x0 (cse_loc l) (bind_typ T))...
 Qed.
@@ -309,23 +283,21 @@ Proof with eauto.
   generalize dependent E.
   dependent induction WfCse; intros; subst; simpl in *.
   1,3,5: loc_transform_cse_ident_eq LocTrans...
-  - apply ok_from_wf_ctx in WfCtx.
-    binds_cases H; subst.
-    + destruct (bind_typ_capt _ _ _ _ WfΓ H0) as [C [R Eq]]; subst.
-      unshelve epose proof (runtime_ctx_binds_loc Γ) as [l [BindsL EqL]]...
-      subst.
-      epose proof (loc_transform_cse_bound_fvar _ _ _ BindsL) as LocTransFvar.
-      epose proof (loc_transform_cse_deterministic _ _ _ _ LocTrans LocTransFvar); subst...
-      destruct ((proj2 (env_typing_inversion _ _ _ _ _ _ EnvTyp BindsL)) H0)...
-    + assert (NotIn: x `notin` dom Γ). {
-        eapply head_not_in_tail...
-        apply binds_In in H1...
-      }
-      erewrite <- env_well_typed_preserves_dom in NotIn...
-      epose proof (loc_transform_cse_unbound_fvar _ _ NotIn) as Ident.
+  - apply uniq_from_wf_ctx in WfCtx.
+    analyze_binds_uniq H; subst.
+    + erewrite <- env_well_typed_preserves_dom in H0...
+      epose proof (loc_transform_cse_unbound_fvar _ _ H0) as Ident.
       epose proof (loc_transform_cse_deterministic _ _ _ _ LocTrans Ident); subst...
       epose proof (loc_transform_result T E) as [T' LocTransT']...
-      eapply loc_transform_ctx_binds in H1...
+      econstructor...
+      eapply loc_transform_ctx_binds_typ in BindsTac...
+    + destruct (bind_typ_capt _ _ _ _ WfΓ BindsTac) as [C [R Eq]]; subst.
+      unshelve epose proof (runtime_ctx_binds_loc Γ _ _ _ _ R) as [l [BindsL EqL]]...
+      subst.
+      assert (uniq E) by (eapply env_well_typed_uniq; eauto).
+      unshelve epose proof (loc_transform_cse_bound_fvar _ _ _ _ BindsL) as LocTransFvar...
+      epose proof (loc_transform_cse_deterministic _ _ _ _ LocTrans LocTransFvar); subst...
+      destruct (proj2 (env_typing_inversion _ _ _ R _ _ EnvTyp BindsL))...
   - epose proof (loc_transform_cse_result Q1 E) as [Q1' LocTransQ1].
     epose proof (loc_transform_cse_result Q2 E) as [Q2' LocTransQ2].
     epose proof (loc_transform_cse_join _ _ _ _ _ LocTransQ1 LocTransQ2) as LocTransJoin.
@@ -335,111 +307,6 @@ Proof with eauto.
     eapply IHWfCse2...
 Qed.
 
-Lemma subcapt_under_loc_transform : forall Γ E S C1 C2 C1' C2',
-  env_well_typed S E Γ ->
-  loc_transform_cse E C1 C1' ->
-  loc_transform_cse E C2 C2' ->
-  subcapt Γ S C1 C2 ->
-  subcapt nil S C1' C2'.
-Proof with eauto*.
-  intros * EnvTyp LocTrans1 LocTrans2 Subcapt.
-  generalize dependent C1'.
-  generalize dependent C2'.
-  generalize dependent E.
-  dependent induction Subcapt; intros.
-  - loc_transform_cse_ident_eq LocTrans2...
-    constructor...
-    eapply loc_transform_cse_wf_nil...
-  - loc_transform_cse_ident_eq LocTrans1...
-    constructor...
-    eapply loc_transform_cse_wf_nil...
-  - assert (X `in` dom E). {
-     epose proof (wf_cse_fvars_from_ctx _ _ _ X H0).
-     erewrite <- env_well_typed_preserves_dom in H1...
-     simpl in *...
-     fsetdec.
-    }
-    dependent induction EnvTyp; simpl in *; try fsetdec.
-    destruct (x == X) eqn:Eq; subst.
-    + inverts LocTrans1.
-      simpl in *.
-      destruct (X == X) eqn:Eq'; subst...
-      inverts LocTrans2.
-      simpl in *.
-      destruct (X == X); subst...
-      loc_transform_cse_ident_eq H9...
-      loc_transform_cse_ident_eq H10...
-    + inverts LocTrans1.
-      simpl in *.
-      destruct (x == X); subst...
-      inverts LocTrans2.
-      simpl in *.
-      destruct (x == X); subst...
-      assert (X `in` dom E) by fsetdec.
-      apply IHEnvTyp...
-      inverts H...
-      rewrite_nil_concat.
-      eapply wf_cse_strengthen...
-      simpl...
-  - unshelve epose proof (loc_transform_cse_ident E (cse_loc l) _) as Ident...
-    epose proof (loc_transform_cse_deterministic _ _ _ _ LocTrans1 Ident); subst...
-    epose proof (loc_transform_cse_deterministic _ _ _ _ LocTrans2 Ident); subst...
-    apply subcapt_reflexivity...
-    inverts H0...
-  - destruct (subcapt_regular _ _ _ _ Subcapt) as [_ [_ [WfR _]]].
-    unshelve epose proof (loc_transform_cse_result R E) as [CR LocCR]...
-    assert (subcapt Γ S (cse_fvar X) R). {
-      eapply subcapt_trans_var...
-      eapply subcapt_reflexivity...
-    }
-    destruct (runtime_ctx_binds_loc _ _ _ _ _ _ EnvTyp H) as [l [BindsL Eq]]; subst.
-    apply subcapt_transitivity with (Q := CR)...
-    loc_transform_cse_ident_eq LocCR...
-    epose proof (loc_transform_cse_bound_fvar _ _ _ BindsL).
-    epose proof (loc_transform_cse_deterministic _ _ _ _ H1 LocTrans1); subst...
-    eapply subcapt_reflexivity...
-    epose proof ((proj2 (env_typing_inversion _ _ _ _ _ _ EnvTyp BindsL)) H).
-    destruct H2 as [R' StoreBinds]...
-  - loc_transform_cse_ident_eq LocTrans1...
-    destruct (subcapt_regular _ _ _ _ Subcapt) as [_ [_ [WfR _]]].
-    unshelve epose proof (loc_transform_cse_result R E) as [CR LocCR]...
-    apply subcapt_transitivity with (Q := CR)...
-    assert (WfS : wf_store_ctx S) by (eapply env_well_typed_store_ctx_wf; eauto).
-    assert (WfRT: wf_typ nil S (R # T)) by (eapply wf_typ_from_wf_store_ctx_nil; eauto).
-    inverts WfRT.
-    loc_transform_cse_ident_eq LocCR...
-    epose proof (wf_cse_empty_means_no_fvars _ _ H2)...
-    eapply subcapt_trans_loc...
-    eapply subcapt_reflexivity...
-  - destruct (loc_transform_cse_result R2 E) as [CR2 LocTransCR2].
-    assert (WfR1 : wf_cse Γ S R1) by applys subcapt_regular Subcapt.
-    destruct (loc_transform_cse_result R1 E) as [CR1 LocTransCR1].
-    assert (C2' = cse_join CR1 CR2); subst. {
-      applys loc_transform_cse_deterministic...
-      eapply loc_transform_cse_join...
-    }
-    apply subcapt_join_inl...
-    eapply loc_transform_cse_wf_nil with (C1 := R2)...
-  - destruct (loc_transform_cse_result R1 E) as [CR1 LocTransCR1].
-    assert (WfR2 : wf_cse Γ S R2) by applys subcapt_regular Subcapt.
-    destruct (loc_transform_cse_result R2 E) as [CR2 LocTransCR2].
-    assert (C2' = cse_join CR1 CR2); subst. {
-      applys loc_transform_cse_deterministic...
-      eapply loc_transform_cse_join...
-    }
-    apply subcapt_join_inr...
-    eapply loc_transform_cse_wf_nil with (C1 := R1)...
-  - assert (WfR1 : wf_cse Γ S R1) by applys subcapt_regular Subcapt1.
-    assert (WfR2 : wf_cse Γ S R2) by applys subcapt_regular Subcapt2.
-    destruct (loc_transform_cse_result R1 E) as [CR1 LocTransCR1].
-    destruct (loc_transform_cse_result R2 E) as [CR2 LocTransCR2].
-    assert (C1' = cse_join CR1 CR2); subst. {
-      applys loc_transform_cse_deterministic...
-      eapply loc_transform_cse_join...
-    }
-    apply subcapt_join_elim...
-Qed.
-
 Lemma subcapt_under_loc_transform_strong : forall Γ Δ Δ' E S C1 C2 C1' C2',
   env_well_typed S E Γ ->
   subcapt (Δ ++ Γ) S C1 C2 ->
@@ -447,32 +314,98 @@ Lemma subcapt_under_loc_transform_strong : forall Γ Δ Δ' E S C1 C2 C1' C2',
   loc_transform_cse E C2 C2' ->
   loc_transform_ctx E Δ Δ' ->
   subcapt Δ' S C1' C2'.
-Proof with eauto*.
+Proof with eauto using loc_transform_cse_wf, loc_transform_ctx_wf, subcapt_reflexivity.
   intros * EnvTyp Subcapt LocTransC1 LocTransC2 LocTransCtx.
+  assert (Uniq : uniq (Δ ++ Γ)) by eauto.
+  assert (WfΓ : wf_ctx Γ S) by (eapply env_well_typed_ctx_wf; eauto).
+  assert (UniqE: uniq E) by (eapply env_well_typed_uniq; eauto).
+  assert (WfS : wf_store_ctx S) by (eapply env_well_typed_store_ctx_wf; eauto).
   generalize dependent C1'.
   generalize dependent C2'.
   generalize dependent E.
   generalize dependent Δ'.
   dependent induction Subcapt; intros.
   - loc_transform_cse_ident_eq LocTransC2...
-    constructor...
-    eapply loc_transform_ctx_wf...
-    eapply loc_transform_cse_wf...
-Admitted.
+  - loc_transform_cse_ident_eq LocTransC1...
+  - inversion H0; subst.
+    rename select (binds _ _ _) into Binds.
+    analyze_binds_uniq Binds; subst.
+    + erewrite <- env_well_typed_preserves_dom in H1...
+      epose proof (loc_transform_cse_unbound_fvar _ _ H1) as Ident.
+      epose proof (loc_transform_cse_deterministic _ _ _ _ LocTransC1 Ident); subst...
+      epose proof (loc_transform_cse_deterministic _ _ _ _ LocTransC2 Ident); subst...
+    + epose proof (bind_typ_capt _ _ _ _ WfΓ BindsTac) as [C [R Eq]]; subst.
+      unshelve epose proof (runtime_ctx_binds_loc Γ _ _ _ _ R) as [l [BindsL EqL]]...
+      subst.
+      unshelve epose proof (loc_transform_cse_bound_fvar _ _ _ UniqE BindsL) as LocTransFvar...
+      epose proof (loc_transform_cse_deterministic _ _ _ _ LocTransC1 LocTransFvar); subst...
+      epose proof (loc_transform_cse_deterministic _ _ _ _ LocTransC2 LocTransFvar); subst...
+  - loc_transform_cse_ident_eq LocTransC1...
+    loc_transform_cse_ident_eq LocTransC2...
+  - analyze_binds_uniq H; subst.
+    + rewrite <- (env_well_typed_preserves_dom _ _ _ EnvTyp) in H0.
+      epose proof (loc_transform_cse_unbound_fvar _ _ H0) as Ident.
+      epose proof (loc_transform_cse_deterministic _ _ _ _ LocTransC1 Ident); subst.
+      epose proof (loc_transform_result (R # T) E) as [R' LocTransR'].
+      epose proof (loc_transform_capt _ _ _ _ LocTransR') as [C0 [R0 [Eq [LocTransR LocTransT]]]]; subst.
+      epose proof (loc_transform_ctx_binds_typ _ _ _ _ _ _ H0 LocTransCtx BindsTac LocTransR')...
+    + unshelve epose proof (runtime_ctx_binds_loc Γ _ _ _ R T) as [l [BindsL EqL]]...
+      subst.
+      unshelve epose proof (loc_transform_cse_bound_fvar _ _ _ UniqE BindsL) as LocTransFvar.
+      epose proof (loc_transform_cse_deterministic _ _ _ _ LocTransC1 LocTransFvar); subst.
+      eapply IHSubcapt...
+      apply loc_transform_cse_ident...
+  - loc_transform_cse_ident_eq LocTransC1...
+    apply subcapt_transitivity with (Q := R).
+    + assert (WfΔ' : wf_ctx Δ' S) by (eapply loc_transform_ctx_wf; eauto).
+      epose proof (wf_typ_from_wf_store_ctx Δ' _ _ _ _ WfS H WfΔ') as Wf.
+      inversion Wf; subst.
+      econstructor...
+    + epose proof (loc_transform_cse_result R E) as [R' LocTransR].
+      epose proof (wf_typ_from_wf_store_ctx_nil _ _ _ _ WfS H) as WfTyp.
+      inversion WfTyp; subst.
+      loc_transform_cse_ident_eq LocTransR. {
+        intros. intro.
+        epose proof (wf_cse_fvars_from_ctx _ _ _ _ H2 H0)...
+        simpl in *. fsetdec.
+      }
+      eapply IHSubcapt...
+  - epose proof (loc_transform_cse_result R1 E) as [R1' LocTransR1].
+    epose proof (loc_transform_cse_result R2 E) as [R2' LocTransR2].
+    epose proof (loc_transform_cse_join _ _ _ _ _ LocTransR1 LocTransR2) as LocTransJoin.
+    epose proof (loc_transform_cse_deterministic _ _ _ _ LocTransC2 LocTransJoin); subst.
+    apply subcapt_join_inl...
+  - epose proof (loc_transform_cse_result R1 E) as [R1' LocTransR1].
+    epose proof (loc_transform_cse_result R2 E) as [R2' LocTransR2].
+    epose proof (loc_transform_cse_join _ _ _ _ _ LocTransR1 LocTransR2) as LocTransJoin.
+    epose proof (loc_transform_cse_deterministic _ _ _ _ LocTransC2 LocTransJoin); subst.
+    apply subcapt_join_inr...
+  - epose proof (loc_transform_cse_result R1 E) as [R1' LocTransR1].
+    epose proof (loc_transform_cse_result R2 E) as [R2' LocTransR2].
+    epose proof (loc_transform_cse_join _ _ _ _ _ LocTransR1 LocTransR2) as LocTransJoin.
+    epose proof (loc_transform_cse_deterministic _ _ _ _ LocTransC1 LocTransJoin); subst.
+    apply subcapt_join_elim...
+Qed.
 
+Lemma loc_transform_ctx_nil : forall E,
+  loc_transform_ctx E nil nil.
+Proof with eauto.
+  intros.
+  induction E...
+  destruct a as [x l]...
+Qed.
 
-Definition no_type_bindings (Γ : ctx) : Prop :=
-  forall X U, ~ binds X (bind_sub U) Γ.
-
-Lemma runtime_ctx_no_type_bindings : forall Γ E S,
+Lemma subcapt_under_loc_transform : forall Γ E S C1 C2 C1' C2',
   env_well_typed S E Γ ->
-  no_type_bindings Γ.
-Proof with eauto*.
-  intros * EnvTyp.
-  unfold no_type_bindings.
-  dependent induction EnvTyp; intros; intro...
-  - inversion H0.
-  - binds_cases H1...
+  loc_transform_cse E C1 C1' ->
+  loc_transform_cse E C2 C2' ->
+  subcapt Γ S C1 C2 ->
+  subcapt nil S C1' C2'.
+Proof with eauto using subcapt_under_loc_transform_strong.
+  intros * EnvTyp LocTransC1 LocTransC2 Subcapt.
+  rewrite_env (nil ++ Γ) in Subcapt.
+  apply (subcapt_under_loc_transform_strong _ _ _ _ _ _ _ _ _ EnvTyp Subcapt LocTransC1 LocTransC2).
+  apply loc_transform_ctx_nil.
 Qed.
 
 (* Lemma subst_ct_invert_fun : forall T U C R D x, *)
@@ -498,7 +431,7 @@ Lemma loc_transform_fun : forall E C1 R1 T1 U,
     loc_transform E R1 R2 /\
     loc_transform E T1 T2 /\
     U = ∀ (C2 # R2) T2.
-Proof with eauto*.
+Proof with eauto.
   intros * LocTrans.
   dependent induction LocTrans; intros; subst; simpl in *.
   - exists C1, R1, T1; repeat split...
@@ -512,18 +445,18 @@ Lemma loc_transform_tfun : forall E R1 T1 U,
     loc_transform E R1 R2 /\
     loc_transform E T1 T2 /\
     U = ∀ [R2] T2.
-Proof with eauto*.
+Proof with eauto.
   intros * LocTrans.
   dependent induction LocTrans; intros; subst; simpl in *.
   - exists R1, T1; split...
-  - destruct (IHLocTrans _ _ eq_refl) as [R2 [T2 [LocTransR LocTransT]]]; subst.
+  - destruct (IHLocTrans _ _ eq_refl) as [R2 [T2 [LocTransR [LocTransT Eq]]]]; subst.
     exists R2, T2; split...
 Qed.
 
 Lemma loc_transform_box : forall E T1 U,
   loc_transform E (typ_box T1) U ->
   exists T2, loc_transform E T1 T2 /\ U = typ_box T2.
-Proof with eauto*.
+Proof with eauto.
   intros * LocTrans.
   dependent induction LocTrans; intros; subst; simpl in *.
   - exists T1; split... 
@@ -531,44 +464,154 @@ Proof with eauto*.
     exists T2; split...
 Qed.
 
-Lemma sub_under_loc_transform : forall Γ E S T1 T2 T1' T2',
+Lemma loc_transform_ctx_cons : forall E Δ Δ' x T T',
+  loc_transform_ctx E Δ Δ' ->
+  loc_transform E T T' ->
+  loc_transform_ctx E ((x, bind_typ T) :: Δ) ((x, bind_typ T') :: Δ').
+Proof with eauto using loc_transform_ctx_binds_typ, loc_transform_ctx_binds_sub.
+  intros * LocTransCtx LocTrans.
+  generalize dependent T'.
+  generalize dependent T.
+  dependent induction LocTransCtx; intros; subst; simpl in *.
+  - inversion LocTrans; subst.
+    constructor...
+  - inversion LocTrans; subst.
+    constructor...
+    simpl.
+    apply IHLocTransCtx...
+Qed.
+
+Lemma loc_transform_open_fresh : forall x E T1 T2,
+  x `notin`A dom E ->
+  loc_transform E T1 T2 ->
+  loc_transform E (open_ct T1 (cse_fvar x)) (open_ct T2 (cse_fvar x)).
+Proof with eauto using loc_transform_ctx_binds_typ, loc_transform_ctx_binds_sub.
+  intros * NotIn LocTrans.
+  generalize dependent x.
+  dependent induction LocTrans; intros; subst; simpl in *.
+  - constructor...
+  - destruct (x == x0); try fsetdec...
+    constructor...
+    Admitted.
+
+Lemma loc_transform_wf : forall Γ Δ Δ' E S T1 T2,
   env_well_typed S E Γ ->
+  wf_ctx (Δ ++ Γ) S ->
+  wf_typ (Δ ++ Γ) S T1 ->
+  loc_transform E T1 T2 ->
+  loc_transform_ctx E Δ Δ' ->
+  wf_typ Δ' S T2.
+Proof with eauto using loc_transform_ctx_wf, loc_transform_cse_wf, loc_transform_ctx_binds_sub.
+  intros * EnvTyp WfCtx WfTyp LocTrans LocTransCtx.
+  assert (WfΓ : wf_ctx Γ S) by (eapply env_well_typed_ctx_wf; eauto).
+  generalize dependent T2.
+  generalize dependent Δ'.
+  generalize dependent E.
+  dependent induction WfTyp; intros; subst; simpl in *.
+  - analyze_binds_uniq H...
+    + erewrite <- env_well_typed_preserves_dom in H0...
+      epose proof (loc_transform_unbound_var _ _ H0).
+      epose proof (loc_transform_deterministic _ _ _ _ LocTrans H); subst...
+      epose proof (loc_transform_result T E) as [T' LocTransT']...
+    + exfalso.
+      epose proof (runtime_ctx_no_type_bindings _ _ _ EnvTyp) as NoTypeBinds.
+      unfold no_type_bindings in NoTypeBinds.
+      specialize (NoTypeBinds X T)...
+  - loc_transform_ident_eq LocTrans...
+  - epose proof (loc_transform_fun _ _ _ _ _ LocTrans) as [C' [R' [T' [LocTransC [LocTransR [LocTransT Eq]]]]]]; subst.
+    pick fresh x and apply wf_typ_arr.
+    eapply IHWfTyp...
+    apply loc_tranform_equiv...
+    eapply (H0 x ltac:(fsetdec) Γ ((x, bind_typ (C # R)) :: Δ)) with (E := E); auto.
+    + constructor...
+    + apply loc_transform_ctx_cons...
+      eapply loc_tranform_equiv...
+    + 
+Admitted.
+
+Lemma sub_under_loc_transform_strong : forall Γ Δ Δ' E S T1 T2 T1' T2',
+  env_well_typed S E Γ ->
+  sub (Δ ++ Γ) S T1 T2 ->
   loc_transform E T1 T1' ->
   loc_transform E T2 T2' ->
-  sub Γ S T1 T2 ->
-  sub nil S T1' T2'.
-Proof with eauto using subcapt_under_loc_transform, loc_transform_pure.
-  intros * EnvTyp LocTrans1 LocTrans2 Sub.
+  loc_transform_ctx E Δ Δ' ->
+  sub Δ' S T1' T2'.
+Proof with eauto using subcapt_under_loc_transform_strong, loc_transform_ctx_binds_typ, loc_transform_ctx_binds_sub, sub_reflexivity, loc_transform_ctx_wf, loc_transform_pure, loc_transform_wf.
+  intros * EnvTyp Sub LocTransC1 LocTransC2 LocTransCtx.
+  assert (Uniq : uniq (Δ ++ Γ)) by eauto.
+  assert (WfΓ : wf_ctx Γ S) by (eapply env_well_typed_ctx_wf; eauto).
+  assert (UniqE: uniq E) by (eapply env_well_typed_uniq; eauto).
+  assert (WfS : wf_store_ctx S) by (eapply env_well_typed_store_ctx_wf; eauto).
   generalize dependent T1'.
   generalize dependent T2'.
   generalize dependent E.
+  generalize dependent Δ'.
   dependent induction Sub; intros.
-  - exfalso. inverts H0.
-    epose proof (runtime_ctx_no_type_bindings _ _ _ EnvTyp) as NoTypeBinds.
-    specialize (NoTypeBinds X T)...
-  - exfalso.
-    epose proof (runtime_ctx_no_type_bindings _ _ _ EnvTyp) as NoTypeBinds.
-    specialize (NoTypeBinds X U)...
-  - unshelve epose proof (loc_transform_capt _ _ _ _ LocTrans1) as [C1' [R1' [Eq1 [LocTransC1 LocTransR1]]]]; subst.
-    unshelve epose proof (loc_transform_capt _ _ _ _ LocTrans2) as [C2' [R2' [Eq2 [LocTransC2 LocTransR2]]]]; subst.
-    destruct ((proj1 (loc_tranform_equiv _ _ _ _ _)) LocTrans1).
-    destruct ((proj1 (loc_tranform_equiv _ _ _ _ _)) LocTrans2).
+  - inversion H0; subst.
+    rename select (binds _ _ _) into Binds.
+    analyze_binds_uniq Binds; subst.
+    + erewrite <- env_well_typed_preserves_dom in H1...
+      epose proof (loc_transform_unbound_var _ _ H1).
+      epose proof (loc_transform_deterministic _ _ _ _ LocTransC1 H2); subst...
+      epose proof (loc_transform_deterministic _ _ _ _ LocTransC2 H2); subst...
+    + exfalso.
+      epose proof (runtime_ctx_no_type_bindings _ _ _ EnvTyp) as NoTypeBinds.
+      unfold no_type_bindings in NoTypeBinds.
+      specialize (NoTypeBinds X T)...
+  - rename select (binds _ _ _) into Binds.
+    analyze_binds_uniq Binds; subst.
+    + erewrite <- (env_well_typed_preserves_dom _ _ _ EnvTyp) in H.
+      epose proof (loc_transform_unbound_var _ _ H).
+      epose proof (loc_transform_deterministic _ _ _ _ LocTransC1 H0); subst.
+      epose proof (loc_transform_result U E) as [U' LocTransU]...
+    + exfalso.
+      epose proof (runtime_ctx_no_type_bindings _ _ _ EnvTyp) as NoTypeBinds.
+      unfold no_type_bindings in NoTypeBinds.
+      specialize (NoTypeBinds X U)...
+  - epose proof (loc_transform_capt _ _ _ _ LocTransC1) as [C1' [R1' [Eq1 [LocTransC1' LocTransR1']]]]; subst.
+    epose proof (loc_transform_capt _ _ _ _ LocTransC2) as [C2' [R2' [Eq2 [LocTransC2' LocTransR2']]]]; subst.
+    destruct ((proj1 (loc_tranform_equiv _ _ _ _ _)) LocTransC1).
+    destruct ((proj1 (loc_tranform_equiv _ _ _ _ _)) LocTransC2).
     constructor...
-  - epose proof (fv_loc_transform_nil _ _ _ _ _ EnvTyp H0 LocTrans1).
-    enough (T2' = typ_top); subst...
-    unshelve epose proof (loc_transform_ident E typ_top _)...
-    epose proof (loc_transform_deterministic _ _ _ _ LocTrans2 H3)...
-  - destruct (loc_transform_fun _ _ _ _ _ LocTrans1) as [C1r [R1r [T1r [LocTransC1 [LocTransR1 [LocTransT1 Eq]]]]]]; subst.
-    destruct (loc_transform_fun _ _ _ _ _ LocTrans2) as [C2r [R2r [T2r [LocTransC2 [LocTransR2 [LocTransT2 Eq']]]]]]; subst.
-    pick fresh x and apply sub_arr; simpl...
-    admit.
-  - destruct (loc_transform_tfun _ _ _ _ LocTrans1) as [R1r [T1r [LocTransR1 [LocTransT1 Eq]]]]; subst.
-    destruct (loc_transform_tfun _ _ _ _ LocTrans2) as [R2r [T2r [LocTransR2 [LocTransT2 Eq']]]]; subst.
-    pick fresh x and apply sub_all; simpl...
-    admit.
-  - epose proof (loc_transform_box _ _ _ LocTrans1) as [T1r [LocTransT1 Eq]]; subst.
-    epose proof (loc_transform_box _ _ _ LocTrans2) as [T2r [LocTransT2 Eq']]; subst.
-    constructor...
-Admitted.
-    eapply subcapt_trans_loc...
-    eapply subcapt_reflexivity...
+  - loc_transform_ident_eq LocTransC2...
+    Admitted.
+
+(* Lemma sub_under_loc_transform : forall Γ E S T1 T2 T1' T2', *)
+(*   env_well_typed S E Γ -> *)
+(*   loc_transform E T1 T1' -> *)
+(*   loc_transform E T2 T2' -> *)
+(*   sub Γ S T1 T2 -> *)
+(*   sub nil S T1' T2'. *)
+(* Proof with eauto using subcapt_under_loc_transform, loc_transform_pure. *)
+(*   intros * EnvTyp LocTrans1 LocTrans2 Sub. *)
+(*   generalize dependent T1'. *)
+(*   generalize dependent T2'. *)
+(*   generalize dependent E. *)
+(*   dependent induction Sub; intros. *)
+(*   - exfalso. inverts H0. *)
+(*     epose proof (runtime_ctx_no_type_bindings _ _ _ EnvTyp) as NoTypeBinds. *)
+(*     specialize (NoTypeBinds X T)... *)
+(*   - exfalso. *)
+(*     epose proof (runtime_ctx_no_type_bindings _ _ _ EnvTyp) as NoTypeBinds. *)
+(*     specialize (NoTypeBinds X U)... *)
+(*   - unshelve epose proof (loc_transform_capt _ _ _ _ LocTrans1) as [C1' [R1' [Eq1 [LocTransC1 LocTransR1]]]]; subst. *)
+(*     unshelve epose proof (loc_transform_capt _ _ _ _ LocTrans2) as [C2' [R2' [Eq2 [LocTransC2 LocTransR2]]]]; subst. *)
+(*     destruct ((proj1 (loc_tranform_equiv _ _ _ _ _)) LocTrans1). *)
+(*     destruct ((proj1 (loc_tranform_equiv _ _ _ _ _)) LocTrans2). *)
+(*     constructor... *)
+(*   - epose proof (fv_loc_transform_nil _ _ _ _ _ EnvTyp H0 LocTrans1). *)
+(*     enough (T2' = typ_top); subst... *)
+(*     unshelve epose proof (loc_transform_ident E typ_top _)... *)
+(*     epose proof (loc_transform_deterministic _ _ _ _ LocTrans2 H3)... *)
+(*   - destruct (loc_transform_fun _ _ _ _ _ LocTrans1) as [C1r [R1r [T1r [LocTransC1 [LocTransR1 [LocTransT1 Eq]]]]]]; subst. *)
+(*     destruct (loc_transform_fun _ _ _ _ _ LocTrans2) as [C2r [R2r [T2r [LocTransC2 [LocTransR2 [LocTransT2 Eq']]]]]]; subst. *)
+(*     pick fresh x and apply sub_arr; simpl... *)
+(*     admit. *)
+(*   - destruct (loc_transform_tfun _ _ _ _ LocTrans1) as [R1r [T1r [LocTransR1 [LocTransT1 Eq]]]]; subst. *)
+(*     destruct (loc_transform_tfun _ _ _ _ LocTrans2) as [R2r [T2r [LocTransR2 [LocTransT2 Eq']]]]; subst. *)
+(*     pick fresh x and apply sub_all; simpl... *)
+(*     admit. *)
+(*   - epose proof (loc_transform_box _ _ _ LocTrans1) as [T1r [LocTransT1 Eq]]; subst. *)
+(*     epose proof (loc_transform_box _ _ _ LocTrans2) as [T2r [LocTransT2 Eq']]; subst. *)
+(*     constructor... *)
+(* Admitted. *)
